Specification SHA2_256: lemmas necessary for HMAC proof

specs/Spec.SHA2_256.fst
@@ -235,7 +235,7 @@ let lemma_update_multi_extend h0 block blocks =
 
 #reset-options "--max_fuel 0 --z3rlimit 100"
 
-val lemma_hash_prepend: (block:bytes{Seq.length block = size_block}) -> (msg:bytes{Seq.length block + Seq.length msg < max_input_len_8}) -> Lemma
+val lemma_hash_prepend_block: (block:bytes{Seq.length block = size_block}) -> (msg:bytes{Seq.length block + Seq.length msg < max_input_len_8}) -> Lemma
   (ensures (let n = Seq.length msg / size_block in
             let (msg_blocks,msg_last) = Seq.split msg (n * size_block) in
             let hash0 = update h_0 block in
@@ -243,7 +243,7 @@ val lemma_hash_prepend: (block:bytes{Seq.length block = size_block}) -> (msg:byt
             let hash2 = update_last hash1 (size_block + (n * size_block)) msg_last in
             finish hash2 == hash (block @| msg)))
 
-let lemma_hash_prepend block msg =
+let lemma_hash_prepend_block block msg =
   let n = Seq.length msg / size_block in
   let (msg_blocks,msg_last) = Seq.split msg (n * size_block) in
   let hash1 = update h_0 block in
@@ -260,6 +260,46 @@ let lemma_hash_prepend block msg =
   assert(n' == n + 1);
   Seq.lemma_eq_intro (msg_last') (msg_last);
   Seq.lemma_eq_intro (msg_blocks') (block @| msg_blocks)
+
+
+#reset-options "--max_fuel 1 --z3rlimit 100"
+
+let lemma_update_multi_empty (h:hash_w) (empty:bytes{Seq.length empty = 0}) : Lemma
+  (ensures (update_multi h empty == h)) = ()
+
+
+#reset-options "--max_fuel 0 --z3rlimit 100"
+
+val lemma_hash_single_prepend_block: (block:bytes{Seq.length block = size_block}) -> (msg:bytes{Seq.length msg = size_hash}) -> Lemma
+  (ensures (let n = Seq.length msg / size_block in
+            let (msg_blocks,msg_last) = Seq.split msg (n * size_block) in
+            let hash0 = update h_0 block in
+            let hash1 = update_last hash0 (size_block + (n * size_block)) msg_last in
+            finish hash1 == hash (block @| msg)))
+
+let lemma_hash_single_prepend_block block msg =
+  let n = Seq.length msg / size_block in
+  let (msg_blocks,msg_last) = Seq.split msg (n * size_block) in
+  let hash1 = update h_0 block in
+  let hash2 = update_multi hash1 msg_blocks in // This is 0
+  assert(Seq.length msg_blocks = 0);
+  lemma_update_multi_empty hash1 msg_blocks;
+  assert(update_multi hash1 msg_blocks == hash1);
+  Seq.lemma_eq_intro (update h_0 block) (update_multi hash1 msg_blocks);
+  assert(hash2 == update h_0 block);
+  let hash3 = update_last hash2 (size_block + (n * size_block)) msg_last in
+  let hash4 = finish hash3 in
+  lemma_update_multi_extend h_0 block msg_blocks;
+  lemma_eq_intro (block @| msg) (block @| msg_blocks @| msg_last);
+  assert(hash2 == update_multi h_0 (block @| msg_blocks));
+  let banana = block @| msg in
+  let n' = Seq.length banana / size_block in
+  let (msg_blocks',msg_last') = Seq.split banana (n' * size_block) in
+  Math.Lemmas.distributivity_add_left n 1 size_block;
+  assert(n' == n + 1);
+  Seq.lemma_eq_intro (msg_last') (msg_last);
+  Seq.lemma_eq_intro (msg_blocks') (block @| msg_blocks)
+
 
 
 //
